
- H(qubit) wendet das **Hadamard-Gate (H)** an:
	- $$ H|0\rangle = \frac{|0\rangle + |1\rangle}{\sqrt{2}} $$
	- H(qubit) wendet das **Hadamard-Gate (H)** an:
	- $$ H|0\rangle = \frac{|0\rangle + |1\rangle}{\sqrt{2}} $$
- - H(qubit) wendet das **Hadamard-Gate (H)** an:
	- $$ H|0\rangle = \frac{|0\rangle + |1\rangle}{\sqrt{2}} $$
- - H(qubit) wendet das **Hadamard-Gate (H)** an:
	- $$ H|0\rangle = \frac{|0\rangle + |1\rangle}{\sqrt{2}} $$
- - H(qubit) wendet das **Hadamard-Gate (H)** an:
	- $$ H|0\rangle = \frac{|0\rangle + |1\rangle}{\sqrt{2}} $$
- - H(qubit) wendet das **Hadamard-Gate (H)** an:
	- $$ H|0\rangle = \frac{|0\rangle + |1\rangle}{\sqrt{2}} $$
- - H(qubit) wendet das **Hadamard-Gate (H)** an:
	- $$ H|0\rangle = \frac{|0\rangle + |1\rangle}{\sqrt{2}} $$
- - H(qubit) wendet das **Hadamard-Gate (H)** an:
	- $$ H|0\rangle = \frac{|0\rangle + |1\rangle}{\sqrt{2}} $$
- - H(qubit) wendet das **Hadamard-Gate (H)** an:
	- $$ H|0\rangle = \frac{|0\rangle + |1\rangle}{\sqrt{2}} $$
- - H(qubit) wendet das **Hadamard-Gate (H)** an:
	- $$ H|0\rangle = \frac{|0\rangle + |1\rangle}{\sqrt{2}} $$
- - H(qubit) wendet das **Hadamard-Gate (H)** an:
	- $$ H|0\rangle = \frac{|0\rangle + |1\rangle}{\sqrt{2}} $$
- - H(qubit) wendet das **Hadamard-Gate (H)** an:
	- $$ H|0\rangle = \frac{|0\rangle + |1\rangle}{\sqrt{2}} $$
- - H(qubit) wendet das **Hadamard-Gate (H)** an:
	- $$ H|0\rangle = \frac{|0\rangle + |1\rangle}{\sqrt{2}} $$
- - H(qubit) wendet das **Hadamard-Gate (H)** an:
	- $$ H|0\rangle = \frac{|0\rangle + |1\rangle}{\sqrt{2}} $$
- - H(qubit) wendet das **Hadamard-Gate (H)** an:
	- $$ H|0\rangle = \frac{|0\rangle + |1\rangle}{\sqrt{2}} $$
	- 